WIP: proving wellformedness

theories/steps.v
@@ -3,24 +3,30 @@ From stbor Require Import lang notation.
 Class Wellformed A := Wf : A → Prop.
 Existing Class Wf.
 
+Definition wf_stack_item (stack: bstack) (clock: time) (β: barriers)
+  : Prop := ∀ si, si ∈ stack.(borrows) →  match si with
+                                          | Uniq t => (t < clock)%nat
+                                          | FnBarrier c => is_Some (β !! c)
+                                          | _ => True
+                                          end.
+
+Definition wf_bor_value (bor: borrow) (clock: time) : Prop :=
+  match bor with
+  | UniqB t | AliasB (Some t) => (t < clock)%nat
+  | _ => True
+  end.
+Definition wf_bor_values (vl: list immediate) σ :=
+  ∀ l bor, (LitV (LitLoc l bor)) ∈ vl → wf_bor_value bor σ.(cclk).
+
 Record state_wf' σ := {
   state_wf_dom : dom (gset loc) σ.(cheap) ≡ dom (gset loc) σ.(cstk);
   state_wf_mem_bor:
-    ∀ l l' bor, σ.(cheap) !! l = Some (LitV (LitLoc l' bor)) →
-      match bor with
-      | UniqB t | AliasB (Some t) => (t < σ.(cclk))%nat
-      | _ => True
-      end;
+    ∀ l l' bor, σ.(cheap) !! l = Some (LitV (LitLoc l' bor)) → wf_bor_value bor σ.(cclk);
   state_wf_stack_frozen:
     ∀ l stack, σ.(cstk) !! l = Some stack →
       match stack.(frozen_since) with Some t => (t < σ.(cclk))%nat | _ => True end;
   state_wf_stack_item:
-    ∀ l stack si, σ.(cstk) !! l = Some stack → si ∈ stack.(borrows) →
-      match si with
-      | Uniq t => (t < σ.(cclk))%nat
-      | FnBarrier c => is_Some (σ.(cbar) !! c)
-      | _ => True
-      end;
+    ∀ l stack, σ.(cstk) !! l = Some stack → wf_stack_item stack σ.(cclk) σ.(cbar)
 }.
 
 Instance state_wf : Wellformed state :=  state_wf'.
@@ -31,7 +37,7 @@ Lemma init_mem_foldr' l n h (m: nat):
   init_mem (l +ₗ m) n h =
   fold_right (λ (i: nat) hi, <[(l +ₗ i):=LitV ☠%V]> hi) h (seq m n).
 Proof.
-  revert l h m. induction n as [|n IHn]; intros l h m; [done|]. simpl. f_equal.
+  revert m. induction n as [|n IHn]; intros m; [done|]. simpl. f_equal.
   by rewrite shift_loc_assoc -(Nat2Z.inj_add m 1) Nat.add_1_r IHn.
 Qed.
 Lemma init_mem_foldr l n h:
@@ -43,7 +49,7 @@ Lemma free_mem_foldr' l n h (m: nat):
   free_mem (l +ₗ m) n h =
   fold_right (λ (i: nat) hi, delete (l +ₗ i) hi) h (seq m n).
 Proof.
-  revert l h m. induction n as [|n IHn]; intros l h m; [done|]. simpl. f_equal.
+  revert m. induction n as [|n IHn]; intros m; [done|]. simpl. f_equal.
   by rewrite shift_loc_assoc -(Nat2Z.inj_add m 1) Nat.add_1_r IHn.
 Qed.
 Lemma free_mem_foldr l n h:
@@ -55,7 +61,7 @@ Lemma init_stacks_foldr' l n h si (m: nat):
   init_stacks (l +ₗ m) n h si =
   fold_right (λ (i: nat) hi, <[(l +ₗ i):=mkBorStack [si] None]> hi) h (seq m n).
 Proof.
-  revert l h m. induction n as [|n IHn]; intros l h m; [done|]. simpl. f_equal.
+  revert m. induction n as [|n IHn]; intros m; [done|]. simpl. f_equal.
   by rewrite shift_loc_assoc -(Nat2Z.inj_add m 1) Nat.add_1_r IHn.
 Qed.
 Lemma init_stacks_foldr l n h si:
@@ -93,41 +99,40 @@ Proof.
 Qed.
 
 (** Alloc *)
-Lemma alloc_step_wf σ σ' e e' efs h0 l bor T:
-  base_step e σ.(cheap) (Some $ AllocEvt l bor T) e' h0 efs →
+Lemma alloc_step_wf σ σ' e e' obs efs h0 l bor T:
+  base_step e σ.(cheap) (Some $ AllocEvt l bor T) obs e' h0 efs →
   instrumented_step h0 σ.(cstk) σ.(cbar) σ.(cclk)
                     (Some $ AllocEvt l bor T)
                   σ'.(cheap) σ'.(cstk) σ'.(cbar) σ'.(cclk) →
   Wf σ → Wf σ'.
 Proof.
-  destruct σ as [h stk bar clk].
-  destruct σ' as [h' stk' bar' clk']. simpl.
+  destruct σ as [h α β clk].
+  destruct σ' as [h' α' β' clk']. simpl.
   intros BS IS WF. inversion BS. clear BS. simplify_eq.
   destruct (tsize T) eqn:Eqs.
   - inversion IS; clear IS; simplify_eq; constructor; simpl.
     + rewrite Eqs /=. apply WF.
-    + move => ?? bor /(state_wf_mem_bor _ WF).
-      destruct bor as [|[]]; simpl; lia.
-    + rewrite Eqs /=.
-      move => ? stack /(state_wf_stack_frozen _ WF).
+    + move=> ?? bor /(state_wf_mem_bor _ WF). destruct bor as [|[]]; simpl; lia.
+    + rewrite Eqs /= => ? stack /(state_wf_stack_frozen _ WF).
       destruct (stack.(frozen_since)); simpl; lia.
-    + rewrite Eqs /=.
-      move => ?? si Eq In. move : (state_wf_stack_item _ WF _ _ _ Eq In).
+    + rewrite Eqs /= => ?? Eq si In.
+      move : (state_wf_stack_item _ WF _ _ Eq _ In).
       destruct si; [simpl; lia|done..].
   - inversion IS; clear IS; simplify_eq; constructor; cbn -[ init_mem].
-    + rewrite Eqs init_stacks_foldr init_mem_foldr. apply foldr_gmap_insert_dom, WF.
-    + intros l1 l2 bor. rewrite init_mem_foldr.
+    + rewrite Eqs init_stacks_foldr init_mem_foldr.
+      apply foldr_gmap_insert_dom, WF.
+    + intros ?? bor. rewrite init_mem_foldr.
       intros [|Eq]%foldr_gmap_insert_lookup; [done|].
       move : (state_wf_mem_bor _ WF _ _ _ Eq).
       destruct bor as [|[]]; simpl; lia.
-    + intros l1 stack. rewrite init_stacks_foldr.
+    + intros ??. rewrite init_stacks_foldr.
       intros [->|Eq]%foldr_gmap_insert_lookup; [done|].
       move : (state_wf_stack_frozen _ WF _ _ Eq).
       destruct stack.(frozen_since); simpl; lia.
-    + intros l1 stack si. rewrite init_stacks_foldr.
-      intros [->|Eq]%foldr_gmap_insert_lookup.
+    + intros ??. rewrite init_stacks_foldr.
+      intros [->|Eq]%foldr_gmap_insert_lookup si.
       * intros ->%elem_of_list_singleton. lia.
-      * move => /(state_wf_stack_item _ WF _ _ _ Eq).
+      * move => /(state_wf_stack_item _ WF _ _ Eq).
         destruct si; [simpl; lia|done..].
 Qed.
 
@@ -149,7 +154,7 @@ Proof.
   revert α.
   induction n as [|n IHn]; intros α; [by move => [->]|]. simpl.
   case lookup => stack /= ; [|done]. case access1 => stack'; [|done].
-  move => /IHn ->. clear. revert α m. induction n as [|n IH]; intros α m.
+  move => /IHn ->. clear. revert m. induction n as [|n IH]; intros m.
   - by rewrite /= shift_loc_0.
   - simpl. f_equal.
     by rewrite shift_loc_assoc -Nat2Z.inj_add -Nat.add_succ_comm Nat2Z.inj_add
@@ -171,18 +176,18 @@ Proof.
 Qed.
 
 (** Dealloc *)
-Lemma dealloc_step_wf σ σ' e e' efs h0 l bor T :
-  base_step e σ.(cheap) (Some $ DeallocEvt l bor T) e' h0 efs →
+Lemma dealloc_step_wf σ σ' e e' obs efs h0 l bor T :
+  base_step e σ.(cheap) (Some $ DeallocEvt l bor T) obs e' h0 efs →
   instrumented_step h0 σ.(cstk) σ.(cbar) σ.(cclk)
                     (Some $ DeallocEvt l bor T)
                   σ'.(cheap) σ'.(cstk) σ'.(cbar) σ'.(cclk) →
   Wf σ → Wf σ'.
 Proof.
-  destruct σ as [h stk bar clk]. destruct σ' as [h' stk' bar' clk']. simpl.
+  destruct σ as [h α β clk]. destruct σ' as [h' α' β' clk']. simpl.
   intros BS IS WF.
   inversion BS. clear BS. simplify_eq.
   inversion IS. clear IS. simplify_eq.
-  rewrite (accessN_dealloc_delete stk bar' l bor (tsize T) stk'); [|done].
+  rewrite (accessN_dealloc_delete α β' l bor (tsize T) α'); [|done].
   constructor; simpl.
   - rewrite free_mem_foldr. apply foldr_gmap_delete_dom, WF.
   - intros ???. rewrite free_mem_foldr.
@@ -190,8 +195,8 @@ Proof.
     apply (state_wf_mem_bor _ WF _ _ _ Eq).
   - intros ?? Eq%foldr_gmap_delete_lookup.
     apply (state_wf_stack_frozen _ WF _ _ Eq).
-  - intros ??? Eq%foldr_gmap_delete_lookup.
-    apply (state_wf_stack_item _ WF _ _ _ Eq).
+  - intros ?? Eq%foldr_gmap_delete_lookup.
+    apply (state_wf_stack_item _ WF _ _ Eq).
 Qed.
 
 (** Copy *)
@@ -204,11 +209,11 @@ Proof.
   - by apply union_subseteq_r.
 Qed.
 
-Lemma accessN_normal_dom α β l bor n kind α' (ND: kind ≠ AccessDealloc) :
+Lemma accessN_dom α β l bor n kind α' (ND: kind ≠ AccessDealloc) :
   accessN α β l bor n kind = Some α' →
   dom (gset loc) α ≡ dom (gset loc) α'.
 Proof.
-  revert α α'. induction n as [|n IH]; intros α α'; [by move => /= [-> //]|].
+  revert α. induction n as [|n IH]; intros α; [by move => /= [-> //]|].
   simpl. destruct (α !! (l +ₗ n)) eqn:Eq; [|done].
   simpl. case access1 => stack' /=; [|done]. intros Eq2.
   have Eq3: dom (gset loc) α' ≡ dom (gset loc) (<[l +ₗ n:=stack']> α).
@@ -216,27 +221,136 @@ Proof.
   rewrite Eq3. symmetry. apply dom_map_insert_is_Some. by eexists.
 Qed.
 
-Lemma copy_step_wf σ σ' e e' efs h0 l bor T :
-  base_step e σ.(cheap) (Some $ CopyEvt l bor T) e' h0 efs →
-  instrumented_step h0 σ.(cstk) σ.(cbar) σ.(cclk)
-                    (Some $ CopyEvt l bor T)
-                  σ'.(cheap) σ'.(cstk) σ'.(cbar) σ'.(cclk) →
-  Wf σ → Wf σ'.
+(** SqSubsetEq for option *)
+Instance option_sqsubseteq `{SqSubsetEq A} : SqSubsetEq (option A) :=
+  λ o1 o2, if o1 is Some x1 return _ then
+              if o2 is Some x2 return _ then x1 ⊑ x2 else False
+           else True.
+Instance option_sqsubseteq_preorder `{SqSubsetEq A} `{!@PreOrder A (⊑)} :
+  @PreOrder (option A) (⊑).
 Proof.
-  destruct σ as [h stk bar clk]. destruct σ' as [h' stk' bar' clk']. simpl.
+  split.
+  - move=>[x|] //. apply (@reflexivity A (⊑) _).
+  - move=>[x|] [y|] [z|] //. apply (@transitivity A (⊑) _).
+Qed.
+Instance option_sqsubseteq_po `{SqSubsetEq A} `{!@PartialOrder A (⊑)} :
+  @PartialOrder (option A) (⊑).
+Proof.
+  split; [apply _|].
+  move => [?|] [?|] ??; [|done|done|done]. f_equal. by apply : anti_symm.
+Qed.
+
+Instance nat_sqsubseteq : SqSubsetEq nat := le.
+Instance nat_sqsubseteq_po : @PartialOrder nat (⊑) := _.
+
+Lemma access1'_item_stack stk bor kind β stk' :
+  access1' stk bor kind β = Some stk' → stk' `suffix_of` stk.
+Proof.
+  revert bor. induction stk as [|si stk IH]; intros bor; simpl; [done|].
+  destruct si; [destruct bor..|].
+  - case_match => [|/IH]; [|by apply suffix_cons_r].
+    case_match => [[<-//]|//].
+  - move => /IH. by apply suffix_cons_r.
+  - destruct kind; [by move => [<-]|..]; move => /IH; by apply suffix_cons_r.
+  - destruct kind; [by move => [<-]|..]; case_match => [[->//]|//].
+  - case_match => [//|/IH]. by apply suffix_cons_r.
+Qed.
+
+Lemma access1_stack β stk stk' bor kind :
+  access1 β stk bor kind = Some stk' →
+  suffix stk'.(borrows) stk.(borrows) ∧ stk'.(frozen_since) ⊑ stk.(frozen_since).
+Proof.
+  rewrite /access1.
+  case (frozen_since _) as [t|] eqn:Eqt; rewrite -Eqt;
+    [destruct kind|]; [by move => [<-]|..];
+    (case access1' as [stk0|] eqn:Eq; [|done]); move => [<-] /=; (split; [|done]);
+    by eapply access1'_item_stack.
+Qed.
+
+Lemma accessN_item_lookup α β l bor n kind α' (ND: kind ≠ AccessDealloc) :
+  accessN α β l bor n kind = Some α' →
+  (∀ (i: nat) stk, (i < n)%nat → α !! (l +ₗ i) = Some stk →
+    α' !! (l +ₗ i) = access1 β stk bor kind) ∧
+  (∀ (l': loc), (∀ (i: nat), (i < n)%nat → l' ≠ l +ₗ i) → α' !! l' = α !! l').
+Proof.
+  revert α. induction n as [|n IH]; intros α; simpl.
+  { move => [<-]. split; intros ??; by [lia|]. }
+  case (α !! (l +ₗ n)) as [stkn|] eqn:Eqn; [|done] => /=.
+  case access1 as [stkn'|] eqn: Eqn'; [|done] => /= Eq3'.
+  have Eq3 : accessN (<[l +ₗ n:=stkn']> α) β l bor n kind = Some α'
+        by destruct kind. clear Eq3'.
+  destruct (IH _ Eq3) as [IH1 IH2]. split.
+  - intros i stk Lt Eqi. case (decide (i = n)) => Eq'; [subst i|].
+    + rewrite Eqi in Eqn. simplify_eq.
+      rewrite Eqn' IH2; [by rewrite lookup_insert|].
+      move => ?? /shift_loc_inj /Z_of_nat_inj ?. by lia.
+    + apply IH1; [lia|]. rewrite lookup_insert_ne; [done|].
+      by move => /shift_loc_inj /Z_of_nat_inj ? //.
+  - intros l' Lt. rewrite IH2.
+    + rewrite lookup_insert_ne; [done|]. move => Eql'. apply (Lt n); by [lia|].
+    + move => ??. apply Lt. lia.
+Qed.
+
+Lemma accessN_stack α β l bor n kind α' (ND: kind ≠ AccessDealloc) :
+  accessN α β l bor n kind = Some α' →
+  ∀ (l: loc) stk', α' !! l = Some stk' → ∃ stk, α !! l = Some stk ∧
+    stk'.(borrows) `suffix_of` stk.(borrows) ∧ stk'.(frozen_since) ⊑ stk.(frozen_since).
+Proof.
+  revert α. induction n as [|n IH]; intros α; [move => /= [->]; naive_solver|].
+  simpl. destruct (α !! (l +ₗ n)) as [stk0|] eqn:Eq; [|done].
+  simpl. destruct (access1 β stk0 bor kind)  as [stk0'|] eqn: Eq1; [|done].
+  simpl. intros Eq2' l' stk'.
+  have Eq2: accessN (<[l +ₗ n:=stk0']> α) β l bor n kind = Some α'
+      by destruct kind. clear Eq2'.
+  case (decide (l' = (l +ₗ n))) => [-> Eq'|?].
+  - exists stk0. split; [done|].
+    have ?: stk0' = stk'.
+    { destruct (accessN_item_lookup _ _ _ _ _ _ _ ND Eq2) as [_ HL].
+      move : Eq'. rewrite HL.
+      - by rewrite lookup_insert => [[->]].
+      - move => ?? /shift_loc_inj /Z_of_nat_inj ?. by lia. } subst stk0'.
+    by eapply access1_stack.
+  - move => /(IH _ Eq2) [stk [Eq' SUFF]]. exists stk. split; [|done].
+    move : Eq'. by rewrite lookup_insert_ne.
+Qed.
+
+Instance elem_of_list_suffix_proper {A : Type} (x:A) :
+  Proper ((suffix) ==> impl) (x ∈).
+Proof. intros l1 l2 [? ->] ?. rewrite elem_of_app. by right. Qed.
+
+Lemma copy_step_wf σ σ' e e' obs efs h0 l bor T vl :
+  base_step e σ.(cheap) (Some $ CopyEvt l bor T vl) obs e' h0 efs →
+  instrumented_step h0 σ.(cstk) σ.(cbar) σ.(cclk)
+                    (Some $ CopyEvt l bor T vl)
+                  σ'.(cheap) σ'.(cstk) σ'.(cbar) σ'.(cclk) →
+  Wf σ → Wf σ' ∧ wf_bor_values vl σ'.
+Proof.
+  destruct σ as [h α β clk]. destruct σ' as [h' α' β' clk']. simpl.
   intros BS IS WF.
   inversion BS. clear BS. simplify_eq.
-  inversion IS. clear IS. simplify_eq.
-  constructor; simpl.
-  - rewrite -(accessN_normal_dom stk bar' l bor (tsize T) AccessRead);
-      [by apply WF|done..].
-  - apply WF.
-  - admit. (* stk' sub of stk *)
-  - admit. (* stk' sub of stk *)
-Abort.
+  inversion IS. clear IS. simplify_eq. split.
+  - constructor; simpl.
+    + rewrite -(accessN_dom α _ l bor (tsize T) AccessRead); [by apply WF|done..].
+    + apply WF.
+    + intros l' stk'.
+      move=> /(accessN_stack α β' l bor (tsize T) AccessRead α' _ _ l' stk') Eq.
+      destruct Eq as [stk [Eq [_ Sub2]]]; [done..|].
+      destruct stk'.(frozen_since) as [t'|]; [|done].
+      have Eq2 := (state_wf_stack_frozen _ WF _ _ Eq).
+      destruct stk.(frozen_since) as [t|]; [|done].
+      eapply le_lt_trans; [by apply Sub2|done].
+    + intros l' stk'.
+      move=> /(accessN_stack α β' l bor (tsize T) AccessRead α' _ _ l' stk') Eq.
+      destruct Eq as [stk [Eq [Sub1 _]]]; [done..|].
+      intros si Ini. apply (state_wf_stack_item _ WF _ _ Eq).
+      move : Ini. by apply elem_of_list_suffix_proper.
+  - intros l' bor' [i Eqi]%elem_of_list_lookup.
+    have Eqbor: h' !! (l +ₗ i) = Some (LitV (LitLoc l' bor')).
+    { rewrite -Eqi. by eapply VALUES, lookup_lt_Some. }
+    by apply (state_wf_mem_bor _ WF _ _ _ Eqbor).
+Qed.
 
 (** Write *)
-
 Lemma write_mem_dom l vl h
   (DEFINED: ∀ i : nat, (i < strings.length vl)%nat → is_Some (h !! (l +ₗ i))) :
   dom (gset loc) (write_mem l vl h) ≡ dom (gset loc) h.
@@ -249,35 +363,58 @@ Proof.
     rewrite (shift_loc_assoc_nat l 1). apply DEFINED. simpl. lia.
 Qed.
 
-Lemma write_step_wf σ σ' e e' efs h0 l bor T :
-  base_step e σ.(cheap) (Some $ WriteEvt l bor T) e' h0 efs →
-  instrumented_step h0 σ.(cstk) σ.(cbar) σ.(cclk)
-                    (Some $ WriteEvt l bor T)
-                  σ'.(cheap) σ'.(cstk) σ'.(cbar) σ'.(cclk) →
-  Wf σ → Wf σ'.
+Lemma write_mem_lookup l vl h :
+  (∀ (i: nat), (i < length vl)%nat → write_mem l vl h !! (l +ₗ i) = vl !! i) ∧
+  (∀ (l': loc), (∀ (i: nat), (i < length vl)%nat → l' ≠ l +ₗ i) →
+    write_mem l vl h !! l' = h !! l').
 Proof.
-  destruct σ as [h stk bar clk]. destruct σ' as [h' stk' bar' clk']. simpl.
-  intros BS IS WF.
+  revert l h. induction vl as [|v vl IH]; move => l h; simpl; split;
+    [intros ?; by lia|done|..].
+  - intros i Lt. admit.
+  - intros l' Lt. destruct (IH (l +ₗ 1) (<[l:=v]> h)) as [IH1 IH2].
+    rewrite IH2.
+    + admit.
+    + admit.
+Abort.
+
+Lemma write_step_wf σ σ' e e' obs efs h0 l bor T vl :
+  base_step e σ.(cheap) (Some $ WriteEvt l bor T vl) obs e' h0 efs →
+  instrumented_step h0 σ.(cstk) σ.(cbar) σ.(cclk)
+                    (Some $ WriteEvt l bor T vl)
+                  σ'.(cheap) σ'.(cstk) σ'.(cbar) σ'.(cclk) →
+  Wf σ → wf_bor_values vl σ → Wf σ'.
+Proof.
+  destruct σ as [h α β clk]. destruct σ' as [h' α' β' clk']. simpl.
+  intros BS IS WF WFvl.
   inversion BS. clear BS. simplify_eq.
   inversion IS. clear IS. simplify_eq.
   constructor; simpl.
-  - rewrite -(accessN_normal_dom stk bar' l bor (tsize T) AccessWrite);
-      [|done..].
+  - rewrite -(accessN_dom α β' l bor (tsize T) AccessWrite); [|done..].
     rewrite write_mem_dom; [by apply WF|done].
   - admit. (* only true if whatever in el is bound in the memory *)
-  - admit. (* stk' sub of stk *)
-  - admit. (* stk' sub of stk *)
+  - intros l' stk'.
+    move => /(accessN_stack α β' l bor (tsize T) AccessWrite α' _ _ l' stk') Eq.
+    destruct Eq as [stk [Eq [_ Sub2]]]; [done..|].
+    destruct stk'.(frozen_since) as [t'|]; [|done].
+    have Eq2 := (state_wf_stack_frozen _ WF _ _ Eq).
+    destruct stk.(frozen_since) as [t|]; [|done].
+    eapply le_lt_trans; [by apply Sub2|done].
+  - intros l' stk'.
+    move => /(accessN_stack α β' l bor (tsize T) AccessWrite α' _ _ l' stk') Eq.
+    destruct Eq as [stk [Eq [Sub1 _]]]; [done..|].
+    intros si Ini. apply (state_wf_stack_item _ WF _ _ Eq).
+    move : Ini. by apply elem_of_list_suffix_proper.
 Abort.
 
 (** Deref *)
-Lemma deref_step_wf σ σ' e e' efs h0 l bor T mut :
-  base_step e σ.(cheap) (Some $ DerefEvt l bor T mut) e' h0 efs →
+Lemma deref_step_wf σ σ' e e' obs efs h0 l bor T mut :
+  base_step e σ.(cheap) (Some $ DerefEvt l bor T mut) obs e' h0 efs →
   instrumented_step h0 σ.(cstk) σ.(cbar) σ.(cclk)
                     (Some $ DerefEvt l bor T mut)
                   σ'.(cheap) σ'.(cstk) σ'.(cbar) σ'.(cclk) →
   Wf σ → Wf σ'.
 Proof.
-  destruct σ as [h stk bar clk]. destruct σ' as [h' stk' bar' clk']. simpl.
+  destruct σ as [h α β clk]. destruct σ' as [h' α' β' clk']. simpl.
   intros BS IS WF.
   inversion BS. clear BS. simplify_eq.
   inversion IS. clear IS. simplify_eq.
@@ -285,80 +422,79 @@ Proof.
 Qed.
 
 (** NewCall *)
-Lemma newcall_step_wf σ σ' e e' efs h0 n :
-  base_step e σ.(cheap) (Some $ NewCallEvt n) e' h0 efs →
+Lemma newcall_step_wf σ σ' e e' obs efs h0 n :
+  base_step e σ.(cheap) (Some $ NewCallEvt n) obs e' h0 efs →
   instrumented_step h0 σ.(cstk) σ.(cbar) σ.(cclk)
                     (Some $ NewCallEvt n)
                   σ'.(cheap) σ'.(cstk) σ'.(cbar) σ'.(cclk) →
   Wf σ → Wf σ'.
 Proof.
-  destruct σ as [h stk bar clk]. destruct σ' as [h' stk' bar' clk']. simpl.
+  destruct σ as [h α β clk]. destruct σ' as [h' α' β' clk']. simpl.
   intros BS IS WF.
   inversion BS. clear BS. simplify_eq.
   inversion IS. clear IS. simplify_eq.
   constructor; simpl; [apply WF..|].
-  intros ??? Eq In. have SI := state_wf_stack_item _ WF _ _ _ Eq In.
+  intros ?? Eq ? In. have SI := state_wf_stack_item _ WF _ _ Eq _ In.
   destruct si; [done..|]. rewrite lookup_insert_is_Some'. by right.
 Qed.
 
 (** EndCall *)
-Lemma endcall_step_wf σ σ' e e' efs h0 n :
-  base_step e σ.(cheap) (Some $ EndCallEvt n) e' h0 efs →
+Lemma endcall_step_wf σ σ' e e' obs efs h0 n :
+  base_step e σ.(cheap) (Some $ EndCallEvt n) obs e' h0 efs →
   instrumented_step h0 σ.(cstk) σ.(cbar) σ.(cclk)
                     (Some $ EndCallEvt n)
                   σ'.(cheap) σ'.(cstk) σ'.(cbar) σ'.(cclk) →
   Wf σ → Wf σ'.
 Proof.
-  destruct σ as [h stk bar clk]. destruct σ' as [h' stk' bar' clk']. simpl.
+  destruct σ as [h α β clk]. destruct σ' as [h' α' β' clk']. simpl.
   intros BS IS WF.
   inversion BS. clear BS. simplify_eq.
   inversion IS. clear IS. simplify_eq.
   constructor; simpl; [apply WF..|].
-  intros ??? Eq In. have SI := state_wf_stack_item _ WF _ _ _ Eq In.
+  intros ?? Eq ? In. have SI := state_wf_stack_item _ WF _ _ Eq _ In.
   destruct si; [done..|]. rewrite lookup_insert_is_Some'. by right.
 Qed.
 
-
 (** Retag *)
-Lemma retag_step_wf σ σ' e e' efs h0 l T kind :
-  base_step e σ.(cheap) (Some $ RetagEvt l T kind) e' h0 efs →
+Lemma retag_step_wf σ σ' e e' obs efs h0 l T kind :
+  base_step e σ.(cheap) (Some $ RetagEvt l T kind) obs e' h0 efs →
   instrumented_step h0 σ.(cstk) σ.(cbar) σ.(cclk)
-                    (Some $ RetagEvt l T kind)
+                    (Some $ RetagEvt l T kind) 
                   σ'.(cheap) σ'.(cstk) σ'.(cbar) σ'.(cclk) →
   Wf σ → Wf σ'.
 Proof.
-  destruct σ as [h stk bar clk]. destruct σ' as [h' stk' bar' clk']. simpl.
+  destruct σ as [h α β clk]. destruct σ' as [h' α' β' clk']. simpl.
   intros BS IS WF.
   inversion BS. clear BS. simplify_eq.
   inversion IS. clear IS. simplify_eq.
   constructor; simpl.
   - admit. (* no change in dom of h' stk' *)
   - admit. (* new bor comes from increasing clk *)
-  - admit. (* new bor comes from increasing clk *)
-  - admit. (* barrier must be in memory *)
+  - admit. (* new frozen comes from increasing clk *)
+  - admit. (* new bor comes from increasing clk, barrier must be in memory *)
 Abort.
 
 (** None event step *)
-Lemma None_step_wf σ σ' e e' efs h0 :
-  base_step e σ.(cheap) None e' h0 efs →
+Lemma None_step_wf σ σ' e e' obs efs h0 :
+  base_step e σ.(cheap) None obs e' h0 efs →
   instrumented_step h0 σ.(cstk) σ.(cbar) σ.(cclk)
                     None
                   σ'.(cheap) σ'.(cstk) σ'.(cbar) σ'.(cclk) →
   Wf σ → Wf σ'.
 Proof.
-  destruct σ as [h stk bar clk]. destruct σ' as [h' stk' bar' clk']. simpl.
+  destruct σ as [h α β clk]. destruct σ' as [h' α' β' clk']. simpl.
   intros BS IS WF.
   inversion BS; clear BS; simplify_eq;
   inversion IS; clear IS; simplify_eq; apply WF.
 Qed.
 
-Lemma head_step_wf σ σ' e e' efs :
-  head_step e σ [] e' σ' efs → Wf σ → Wf σ'.
+Lemma head_step_wf σ σ' e e' obs efs :
+  head_step e σ obs e' σ' efs → Wf σ → Wf σ'.
 Proof.
   intros HS WF. inversion HS. simplify_eq. destruct oevent as [[]|].
   - eapply alloc_step_wf; eauto.
   - eapply dealloc_step_wf; eauto.
-  - admit.
+  - eapply copy_step_wf; eauto.
   - admit.
   - eapply deref_step_wf; eauto.
   - eapply newcall_step_wf; eauto.
